thy/Bitmagic/Numberwang_Ln.thy
@@ -1,12 +1,13 @@
 theory Numberwang_Ln
-imports NumberWangCebewee
+imports NumberWangCebewee IPv4Addr
 begin
 
-lemma ipv4range_prefix_intersect: " \<not> ipv4range_set_from_prefix b2 m2 \<subseteq> ipv4range_set_from_prefix b1 m1 \<Longrightarrow>
-       \<not> ipv4range_set_from_prefix b1 m1 \<subseteq> ipv4range_set_from_prefix b2 m2 \<Longrightarrow>
-       ipv4range_set_from_prefix b1 m1 \<inter> ipv4range_set_from_prefix b2 m2 = {}"
-apply(simp add: ipv4range_set_from_prefix_eq_ip4_set)
-using ip4_set_notsubset_empty_inter by presburger
+(*TODO: move to IpAddresses or somewhere*)
+lemma ipv4range_prefix_intersect: " \<not> ipset_from_cidr b2 m2 \<subseteq> ipset_from_cidr b1 m1 \<Longrightarrow>
+       \<not> ipset_from_cidr b1 m1 \<subseteq> ipset_from_cidr b2 m2 \<Longrightarrow>
+       ipset_from_cidr b1 m1 \<inter> ipset_from_cidr b2 m2 = {}"
+apply(simp add: ipv4range_set_from_prefix_eq_ip_cidr_set)
+using ip_cidr_set_notsubset_empty_inter by blast
 
 
 (*
